flatten the values in memory and see what we can do
in the RustBelt paper, it says "Values only include the most basic kinds of data"
and that "There are no literals for products or sums as these only exist in memory,
represented by sequences of values
and tagged unions, respectively."
But since I want to add records,
I don't know how to represent 'rcons'
(record cons, like the constructor of lists with a field name in the front)
when the field name cover the first part of the values (think of a pair)
after I change the points-to assertion to the flattened ones,
I realize that if I have a (rcons l (t1,t2) t3)
I still don't have a 'pair value' so I can't express them as value

theories/lang/heap.v
@@ -40,19 +40,31 @@ Section definitions.
              (l : loc) (q : Qp) (v: val) : iProp Σ :=
     own heap_name (◯ {[ l := (q, to_lock_stateR st, to_agree v) ]}).
 
-  Definition heap_mapsto_def (l : loc) (q : Qp) (v: val) : iProp Σ :=
+  Definition heap_mapsto_simple_def (l : loc) (q : Qp) (v: val) : iProp Σ :=
     heap_mapsto_st (RSt 0) l q v.
-  Definition heap_mapsto_aux : seal (@heap_mapsto_def). Proof. by eexists. Qed.
-  Definition heap_mapsto := unseal heap_mapsto_aux.
-  Definition heap_mapsto_eq : @heap_mapsto = @heap_mapsto_def :=
-    seal_eq heap_mapsto_aux.
-
+  Definition heap_mapsto_simple_aux : seal (@heap_mapsto_simple_def). Proof. by eexists. Qed.
+  Definition heap_mapsto_simple := unseal heap_mapsto_simple_aux.
+  Definition heap_mapsto_simple_eq : @heap_mapsto_simple = @heap_mapsto_simple_def :=
+    seal_eq heap_mapsto_simple_aux.
+  Fixpoint flattenv v := match v with
+    | RecordVCons l v1 v2 => flattenv v1 ++ flattenv v2
+    | v => [v]
+  end.
+  Fixpoint flatten vl := match vl with
+    | [] => []
+    | v :: vl => flattenv v ++ flatten vl
+  end.
+  Definition heap_mapsto (l : loc) (q : Qp) (v: val) : iProp Σ :=
+    ([∗ list] i ↦ v ∈ (flattenv v), heap_mapsto_simple (l +ₗ i) q v).
+  Definition heap_mapsto_vec_simple l q vl : iProp Σ :=
+      ([∗ list] i ↦ v ∈ vl, heap_mapsto_simple (l +ₗ i) q v)%I.
   Definition heap_mapsto_vec (l : loc) (q : Qp) (vl : list val) : iProp Σ :=
-    ([∗ list] i ↦ v ∈ vl, heap_mapsto (l +ₗ i) q v)%I.
+    ([∗ list] i ↦ v ∈ (flatten vl), heap_mapsto_simple (l +ₗ i) q v)%I.
 
   Fixpoint inter (i0 : Z) (n : nat) : gmapR Z (exclR unitO) :=
     match n with O => ∅ | S n => <[i0 := Excl ()]>(inter (i0+1) n) end.
 
+  (* freeable is the Dealloc in the paper *)
   Definition heap_freeable_def (l : loc) (q : Qp) (n: nat) : iProp Σ :=
     own heap_freeable_name (◯ {[ l.1 := (q, inter (l.2) n) ]}).
   Definition heap_freeable_aux : seal (@heap_freeable_def). Proof. by eexists. Qed.
@@ -70,18 +82,31 @@ Global Typeclasses Opaque heap_mapsto heap_freeable heap_mapsto_vec.
 Global Instance: Params (@heap_mapsto) 4 := {}.
 Global Instance: Params (@heap_freeable) 5 := {}.
 
+Notation "l ↦s{ q } v" := (heap_mapsto_simple l q v)
+  (at level 20, q at level 50, format "l  ↦s{ q }  v") : bi_scope.
 Notation "l ↦{ q } v" := (heap_mapsto l q v)
   (at level 20, q at level 50, format "l  ↦{ q }  v") : bi_scope.
+
 Notation "l ↦ v" := (heap_mapsto l 1 v) (at level 20) : bi_scope.
+Notation "l ↦s v" := (heap_mapsto_simple l 1 v) (at level 20) : bi_scope.
+
+Notation "l ↦∗s{ q } vl" := (heap_mapsto_vec_simple l q vl)
+  (at level 20, q at level 50, format "l  ↦∗s{ q }  vl") : bi_scope.
 
 Notation "l ↦∗{ q } vl" := (heap_mapsto_vec l q vl)
   (at level 20, q at level 50, format "l  ↦∗{ q }  vl") : bi_scope.
 Notation "l ↦∗ vl" := (heap_mapsto_vec l 1 vl) (at level 20) : bi_scope.
+Notation "l ↦∗s vl" := (heap_mapsto_vec_simple l 1 vl) (at level 20) : bi_scope.
+
+Notation "l ↦∗s{ q }: P" := (∃ vl, l ↦∗s{ q } vl ∗ P vl)%I
+  (at level 20, q at level 50, format "l  ↦∗s{ q }:  P") : bi_scope.
 
 Notation "l ↦∗{ q }: P" := (∃ vl, l ↦∗{ q } vl ∗ P vl)%I
   (at level 20, q at level 50, format "l  ↦∗{ q }:  P") : bi_scope.
 Notation "l ↦∗: P " := (∃ vl, l ↦∗ vl ∗ P vl)%I
   (at level 20, format "l  ↦∗:  P") : bi_scope.
+Notation "l ↦∗s: P " := (∃ vl, l ↦∗s vl ∗ P vl)%I
+  (at level 20, format "l  ↦∗s:  P") : bi_scope.
 
 Notation "†{ q } l … n" := (heap_freeable l q n)
   (at level 20, q at level 50, format "†{ q } l … n") : bi_scope.
@@ -113,16 +138,40 @@ Section heap.
 
   (** General properties of mapsto and freeable *)
   Global Instance heap_mapsto_timeless l q v : Timeless (l↦{q}v).
-  Proof. rewrite heap_mapsto_eq /heap_mapsto_def. apply _. Qed.
+  Proof. rewrite /heap_mapsto heap_mapsto_simple_eq. apply _.
+  Qed.
+
+  Global Instance heap_mapsto_simple_timeless l q v : Timeless (l↦s{q}v).
+  Proof. rewrite heap_mapsto_simple_eq. apply _.
+  Qed.
+
+  Global Instance heap_mapsto_simple_fractional l v: Fractional (λ q, l ↦s{q} v)%I.
+  Proof.
+    intros p q.
+    by rewrite heap_mapsto_simple_eq 
+      -own_op -auth_frag_op singleton_op -pair_op agree_idemp.
+  Qed.
 
   Global Instance heap_mapsto_fractional l v: Fractional (λ q, l ↦{q} v)%I.
   Proof.
     intros p q.
-    by rewrite heap_mapsto_eq -own_op -auth_frag_op singleton_op -pair_op agree_idemp.
+    rewrite /heap_mapsto -big_sepL_sep.
+    (* rewrite in func body? seems impossible. well it is possible *)
+    by setoid_rewrite (fractional (Φ := λ q, _ ↦s{q} _)%I).
   Qed.
+
   Global Instance heap_mapsto_as_fractional l q v:
     AsFractional (l ↦{q} v) (λ q, l ↦{q} v)%I q.
   Proof. split; first done. apply _. Qed.
+
+  Global Instance heap_mapsto_simple_as_fractional l q v:
+  AsFractional (l ↦s{q} v) (λ q, l ↦s{q} v)%I q.
+  Proof. split; first done. apply _. Qed.
+
+  Global Instance frame_mapsto_simple p l v q1 q2 RES :
+  FrameFractionalHyps p (l ↦s{q1} v) (λ q, l ↦s{q} v)%I RES q1 q2 →
+  Frame p (l ↦s{q1} v) (l ↦s{q2} v) RES | 5.
+Proof. apply: frame_fractional. Qed.
 
   Global Instance frame_mapsto p l v q1 q2 RES :
     FrameFractionalHyps p (l ↦{q1} v) (λ q, l ↦{q} v)%I RES q1 q2 →
@@ -130,64 +179,163 @@ Section heap.
   Proof. apply: frame_fractional. Qed.
 
   Global Instance heap_mapsto_vec_timeless l q vl : Timeless (l ↦∗{q} vl).
-  Proof. rewrite /heap_mapsto_vec. apply _. Qed.
+  Proof. rewrite /heap_mapsto_vec heap_mapsto_simple_eq. apply _. Qed.
+
+  Global Instance heap_mapsto_vec_simple_timeless l q vl : Timeless (l ↦∗s{q} vl).
+  Proof. rewrite /heap_mapsto_vec_simple. apply _. Qed.
 
   Global Instance heap_mapsto_vec_fractional l vl: Fractional (λ q, l ↦∗{q} vl)%I.
   Proof.
     intros p q. rewrite /heap_mapsto_vec -big_sepL_sep.
-    by setoid_rewrite (fractional (Φ := λ q, _ ↦{q} _)%I).
+    by setoid_rewrite (fractional (Φ := λ q, _ ↦s{q} _)%I).
   Qed.
+
+  Global Instance heap_mapsto_vec_simple_fractional l vl: Fractional (λ q, l ↦∗s{q} vl)%I.
+  Proof.
+    intros p q. rewrite /heap_mapsto_vec_simple -big_sepL_sep.
+    by setoid_rewrite (fractional (Φ := λ q, _ ↦s{q} _)%I).
+  Qed.
+
   Global Instance heap_mapsto_vec_as_fractional l q vl:
     AsFractional (l ↦∗{q} vl) (λ q, l ↦∗{q} vl)%I q.
+  Proof. split; first done. apply _. Qed.
+
+  Global Instance heap_mapsto_vec_simple_as_fractional l q vl:
+    AsFractional (l ↦∗s{q} vl) (λ q, l ↦∗s{q} vl)%I q.
   Proof. split; first done. apply _. Qed.
 
   Global Instance heap_freeable_timeless q l n : Timeless (†{q}l…n).
   Proof. rewrite heap_freeable_eq /heap_freeable_def. apply _. Qed.
 
-  Lemma heap_mapsto_agree l q1 q2 v1 v2 : l ↦{q1} v1 ∗ l ↦{q2} v2 ⊢ ⌜v1 = v2⌝.
+  Lemma heap_mapsto_agree l q1 q2 v1 v2 : l ↦s{q1} v1 ∗ l ↦s{q2} v2 ⊢ ⌜v1 = v2⌝.
   Proof.
-    rewrite heap_mapsto_eq -own_op -auth_frag_op own_valid discrete_valid.
+    rewrite heap_mapsto_simple_eq -own_op -auth_frag_op own_valid discrete_valid.
     eapply pure_elim; [done|]=> /auth_frag_valid /=.
     rewrite singleton_op -pair_op singleton_valid=> -[? /to_agree_op_inv_L->]; eauto.
+  Qed.
+
+  Lemma heap_mapsto_vec_eq l q vl : l ↦∗s{q} (flatten vl) ⊣⊢ l ↦∗{q} vl.
+  Proof.
+    by rewrite /heap_mapsto_vec /heap_mapsto_vec_simple.
   Qed.
 
   Lemma heap_mapsto_vec_nil l q : l ↦∗{q} [] ⊣⊢ True.
   Proof. by rewrite /heap_mapsto_vec. Qed.
 
-  Lemma heap_mapsto_vec_app l q vl1 vl2 :
-    l ↦∗{q} (vl1 ++ vl2) ⊣⊢ l ↦∗{q} vl1 ∗ (l +ₗ length vl1) ↦∗{q} vl2.
+  Lemma flatten_dist vl1 vl2 : flatten (vl1 ++ vl2) = flatten vl1 ++ flatten vl2.
   Proof.
-    rewrite /heap_mapsto_vec big_sepL_app.
+    induction vl1; auto.
+    rewrite <-app_comm_cons.
+    simpl. rewrite <-app_assoc. f_equiv. apply IHvl1.
+  Qed.
+
+  Lemma flatten_size vl : length (flatten vl) = list_ty_size vl.
+  Proof.
+    induction vl; auto. simpl. rewrite lty_cons.
+    rewrite app_length IHvl. f_equal.
+    induction a; try done. simpl. rewrite app_length. naive_solver.
+  Qed.
+
+  Lemma heap_mapsto_vec_app l q vl1 vl2 :
+    l ↦∗{q} (vl1 ++ vl2) ⊣⊢ l ↦∗{q} vl1 ∗ (l +ₗ list_ty_size vl1) ↦∗{q} vl2.
+  Proof.
+    rewrite /heap_mapsto_vec flatten_dist big_sepL_app.
+    do 2 f_equiv. intros k v. by rewrite flatten_size shift_loc_assoc_nat.
+  Qed.
+
+  (* this lemma can't hold now, because we added compound values like records *)
+  Lemma heap_mapsto_vec_singleton l q v : l ↦∗{q} [v] ⊣⊢ l ↦{q} v.
+  Proof.
+    by rewrite /heap_mapsto_vec /flatten /heap_mapsto app_nil_r. 
+  Qed.
+  Lemma lty_size_singleton v : list_ty_size [v] = val_size v.
+    Proof. by rewrite /list_ty_size /=. 
+  Qed.
+  Lemma heap_mapsto_vec_cons l q v vl:
+    l ↦∗{q} (v :: vl) ⊣⊢ l ↦{q} v ∗ (l +ₗ val_size v) ↦∗{q} vl.
+  Proof.
+    by rewrite (heap_mapsto_vec_app l q [v] vl) 
+      lty_size_singleton heap_mapsto_vec_singleton.
+  Qed.
+
+  Lemma heap_mapsto_vec_nil_s l q : l ↦∗s{q} [] ⊣⊢ True.
+  Proof. by rewrite /heap_mapsto_vec_simple. Qed.
+
+  Lemma heap_mapsto_vec_app_s l q vl1 vl2 :
+    l ↦∗s{q} (vl1 ++ vl2) ⊣⊢ l ↦∗s{q} vl1 ∗ (l +ₗ length vl1) ↦∗s{q} vl2.
+  Proof.
+    rewrite /heap_mapsto_vec_simple big_sepL_app.
     do 2 f_equiv. intros k v. by rewrite shift_loc_assoc_nat.
   Qed.
 
-  Lemma heap_mapsto_vec_singleton l q v : l ↦∗{q} [v] ⊣⊢ l ↦{q} v.
-  Proof. by rewrite /heap_mapsto_vec /= shift_loc_0 right_id. Qed.
+  Lemma heap_mapsto_vec_singleton_s l q v : l ↦∗s{q} [v] ⊣⊢ l ↦s{q} v.
+  Proof. by rewrite /heap_mapsto_vec_simple /= shift_loc_0 right_id. Qed.
 
-  Lemma heap_mapsto_vec_cons l q v vl:
-    l ↦∗{q} (v :: vl) ⊣⊢ l ↦{q} v ∗ (l +ₗ 1) ↦∗{q} vl.
+  Lemma heap_mapsto_vec_cons_s l q v vl:
+    l ↦∗s{q} (v :: vl) ⊣⊢ l ↦s{q} v ∗ (l +ₗ 1) ↦∗s{q} vl.
   Proof.
-    by rewrite (heap_mapsto_vec_app l q [v] vl) heap_mapsto_vec_singleton.
+    by rewrite (heap_mapsto_vec_app_s l q [v] vl) heap_mapsto_vec_singleton_s.
   Qed.
-
-  Lemma heap_mapsto_vec_op l q1 q2 vl1 vl2 :
+  Lemma flattenv_noemp v : flattenv v ≠ [].
+  Proof.
+    induction v; try done. simpl. intro H.
+    by destruct (app_eq_nil _ _ H).
+  Qed.
+  Lemma flatten_emp vl : [] = flatten vl ↔ vl = [].
+  Proof.
+    assert (∀ v, flattenv v ≠ []) by apply flattenv_noemp.
+    split.
+    - rewrite /flatten. destruct vl; first done. intros. symmetry in H0. 
+      destruct (app_eq_nil _ _ H0).
+      destruct (H v). done.
+    - intros. by rewrite /flatten H0.
+  Qed.
+  (* it's also very hard adapting the following lemma 
+    I know! I can keep the original mapsto-vec and the related lemmas
+  *)
+  Lemma heap_mapsto_vec_op_s l q1 q2 vl1 vl2 :
     length vl1 = length vl2 →
-    l ↦∗{q1} vl1 ∗ l ↦∗{q2} vl2 ⊣⊢ ⌜vl1 = vl2⌝ ∧ l ↦∗{q1+q2} vl1.
+    l ↦∗s{q1} vl1 ∗ l ↦∗s{q2} vl2 ⊣⊢ ⌜vl1 = vl2⌝ ∧ l ↦∗s{q1+q2} vl1.
   Proof.
     intros Hlen%Forall2_same_length. apply (anti_symm (⊢)).
     - revert l. induction Hlen as [|v1 v2 vl1 vl2 _ _ IH]=> l.
-      { rewrite !heap_mapsto_vec_nil. iIntros "_"; auto. }
-      rewrite !heap_mapsto_vec_cons. iIntros "[[Hv1 Hvl1] [Hv2 Hvl2]]".
+      { rewrite !heap_mapsto_vec_nil_s. iIntros "_"; auto. }
+      rewrite !heap_mapsto_vec_cons_s. iIntros "[[Hv1 Hvl1] [Hv2 Hvl2]]".
       iDestruct (IH (l +ₗ 1) with "[$Hvl1 $Hvl2]") as "[% $]"; subst.
       rewrite (inj_iff (.:: vl2)).
       iDestruct (heap_mapsto_agree with "[$Hv1 $Hv2]") as %<-.
-      iSplit; first done. iFrame.
+      iSplit; first done. iFrame. (* isn't there a global instance? *)
     - by iIntros "[% [$ Hl2]]"; subst.
   Qed.
 
-  Lemma heap_mapsto_pred_op l q1 q2 n (Φ : list val → iProp Σ) :
+  Lemma heap_mapsto_vec_op l q1 q2 vl1 vl2 :
+    list_ty_size vl1 = list_ty_size vl2 →
+    l ↦∗{q1} vl1 ∗ l ↦∗{q2} vl2 ⊣⊢ ⌜flatten vl1 = flatten vl2⌝ ∧ l ↦∗{q1+q2} vl1.
+  Proof.
+    (* beautiful! *)
+    rewrite <-(flatten_size vl1), <-(flatten_size vl2).
+    intros.
+    by rewrite -!heap_mapsto_vec_eq heap_mapsto_vec_op_s.
+  Qed.
+
+  Lemma heap_mapsto_pred_op_s l q1 q2 n (Φ : list val → iProp Σ) :
     (∀ vl, Φ vl -∗ ⌜length vl = n⌝) →
-    l ↦∗{q1}: Φ ∗ l ↦∗{q2}: (λ vl, ⌜length vl = n⌝) ⊣⊢ l ↦∗{q1+q2}: Φ.
+    l ↦∗s{q1}: Φ ∗ l ↦∗s{q2}: (λ vl, ⌜length vl = n⌝) ⊣⊢ l ↦∗s{q1+q2}: Φ.
+  Proof.
+    intros Hlen. iSplit.
+    - iIntros "[Hmt1 Hmt2]".
+      iDestruct "Hmt1" as (vl) "[Hmt1 Hown]". iDestruct "Hmt2" as (vl') "[Hmt2 %]".
+      iDestruct (Hlen with "Hown") as %?.
+      iCombine "Hmt1" "Hmt2" as "Hmt". rewrite heap_mapsto_vec_op_s; last congruence.
+      iDestruct "Hmt" as "[_ Hmt]". iExists vl. by iFrame.
+    - iIntros "Hmt". iDestruct "Hmt" as (vl) "[[Hmt1 Hmt2] Hown]".
+      iDestruct (Hlen with "Hown") as %?.
+      iSplitL "Hmt1 Hown"; iExists _; by iFrame.
+  Qed.
+
+  Lemma heap_mapsto_pred_op l q1 q2 n (Φ : list val → iProp Σ) :
+  (∀ vl, Φ vl -∗ ⌜list_ty_size vl = n⌝) →
+  l ↦∗{q1}: Φ ∗ l ↦∗{q2}: (λ vl, ⌜list_ty_size vl = n⌝) ⊣⊢ l ↦∗{q1+q2}: Φ.
   Proof.
     intros Hlen. iSplit.
     - iIntros "[Hmt1 Hmt2]".
@@ -216,11 +364,14 @@ Section heap.
 
   Lemma heap_mapsto_vec_combine l q vl :
     vl ≠ [] →
-    l ↦∗{q} vl ⊣⊢ own heap_name (◯ [^op list] i ↦ v ∈ vl,
+    l ↦∗{q} vl ⊣⊢ own heap_name (◯ [^op list] i ↦ v ∈ (flatten vl),
       {[l +ₗ i := (q, Cinr 0%nat, to_agree v)]}).
   Proof.
-    rewrite /heap_mapsto_vec heap_mapsto_eq /heap_mapsto_def /heap_mapsto_st=>?.
+    rewrite /heap_mapsto_vec heap_mapsto_simple_eq /heap_mapsto_simple_def /heap_mapsto_st=>?.
     rewrite (big_opL_commute auth_frag) big_opL_commute1 //.
+    rewrite /flatten. intro H. destruct vl; try done.
+    assert (flattenv v ≠ []) by apply flattenv_noemp.
+    by destruct (app_eq_nil _ _ H).
   Qed.
 
   Global Instance heap_mapsto_pred_fractional l (P : list val → iProp Σ):
@@ -231,8 +382,12 @@ Section heap.
       iSplitL "Hown1"; eauto.
     - iIntros "[H1 H2]". iDestruct "H1" as (vl1) "[Hown1 #HP1]".
       iDestruct "H2" as (vl2) "[Hown2 #HP2]".
-      set (ll := min (length vl1) (length vl2)).
-      rewrite -[vl1](firstn_skipn ll) -[vl2](firstn_skipn ll) 2!heap_mapsto_vec_app.
+      set (ll := min (list_ty_size vl1) (list_ty_size vl2)).
+      (* 还能这样rewrite的！ *)
+      admit.
+      (* we might need to introduce a few lemmas about flatten with take/drop*)
+  Admitted.
+      (* rewrite -[vl1](firstn_skipn ll) -[vl2](firstn_skipn ll) 2!heap_mapsto_vec_app.
       iDestruct "Hown1" as "[Hown1 _]". iDestruct "Hown2" as "[Hown2 _]".
       iCombine "Hown1" "Hown2" as "Hown". rewrite heap_mapsto_vec_op; last first.
       { rewrite !firstn_length. subst ll.
@@ -245,7 +400,7 @@ Section heap.
       + iClear "HP1". rewrite Hl take_ge; last first.
         { rewrite -Heq /ll. done. }
         rewrite drop_ge; first by rewrite app_nil_r. by rewrite -Heq.
-  Qed.
+  Qed. *)
   Global Instance heap_mapsto_pred_as_fractional l q (P : list val → iProp Σ):
     (∀ vl, Persistent (P vl)) → AsFractional (l ↦∗{q}: P) (λ q, l ↦∗{q}: P)%I q.
   Proof. split; first done. apply _. Qed.
@@ -382,6 +537,10 @@ Section heap.
     rewrite heap_freeable_eq /heap_freeable_def heap_mapsto_vec_combine //; last first.
     { destruct (Z.to_nat n); done. }
     iFrame. 
+    replace (flatten (repeat (LitV LitPoison) (Z.to_nat n)))
+      with (repeat (LitV LitPoison) (Z.to_nat n)); first done.
+    set (n' := Z.to_nat n).
+    induction n'; first done. simpl. f_equal. apply IHn'.
   Qed.
 
   Lemma heap_free_vs σ l vl :
@@ -405,8 +564,8 @@ Section heap.
   Qed.
 
   Lemma heap_free σ l vl (n : Z) :
-    n = length vl →
-    heap_ctx σ -∗ l ↦∗ vl -∗ †l…(length vl)
+    n = list_ty_size vl →
+    heap_ctx σ -∗ l ↦∗ vl -∗ †l…(list_ty_size vl)
     ==∗ ⌜0 < n⌝ ∗ ⌜∀ m, is_Some (σ !! (l +ₗ m)) ↔ (0 ≤ m < n)⌝ ∗
         heap_ctx (free_mem l (Z.to_nat n) σ).
   Proof.
@@ -418,13 +577,18 @@ Section heap.
     { move: (Hv (l.1)). rewrite Hl. by intros [??]. }
     assert (vl ≠ []).
     { intros ->. by destruct (REL (l.1) (1%Qp, ∅)) as [[] ?]. }
-    assert (0 < n) by (subst n; by destruct vl).
+    assert (0 < n). {
+      subst n.
+      destruct vl; first done. rewrite lty_cons.
+      assert (val_size v >= 1) by apply val_gt1. lia.
+    }
     iMod (heap_free_vs with "[Hmt Hvalσ]") as "Hvalσ".
     { rewrite heap_mapsto_vec_combine //. iFrame. }
     iMod (own_update_2 with "HhF Hf") as "HhF".
     { apply auth_update_dealloc, (delete_singleton_local_update _ _ _). }
     iModIntro; subst. repeat iSplit;  eauto using heap_freeable_is_Some.
     iExists _. subst. rewrite Nat2Z.id. iFrame.
+    rewrite flatten_size.
     eauto using heap_freeable_rel_free_mem.
   Qed.
 
@@ -475,32 +639,32 @@ Section heap.
     apply prod_local_update_1, prod_local_update_2, csum_local_update_r.
     apply nat_local_update; lia.
   Qed.
-
+  (* how to change? *)
   Lemma heap_read σ l q v :
-    heap_ctx σ -∗ l ↦{q} v -∗ ∃ n, ⌜σ !! l = Some (RSt n, v)⌝.
+    heap_ctx σ -∗ l ↦s{q} v -∗ ∃ n, ⌜σ !! l = Some (RSt n, v)⌝.
   Proof.
     iDestruct 1 as (hF) "(Hσ & HhF & REL)". iIntros "Hmt".
-    rewrite heap_mapsto_eq.
+    rewrite heap_mapsto_simple_eq.
     iDestruct (heap_mapsto_lookup with "Hσ Hmt") as %[n Hσl]; eauto.
   Qed.
 
   Lemma heap_read_1 σ l v :
-    heap_ctx σ -∗ l ↦ v -∗ ⌜σ !! l = Some (RSt 0, v)⌝.
+    heap_ctx σ -∗ l ↦s v -∗ ⌜σ !! l = Some (RSt 0, v)⌝.
   Proof.
     iDestruct 1 as (hF) "(Hσ & HhF & REL)". iIntros "Hmt".
-    rewrite heap_mapsto_eq.
+    rewrite heap_mapsto_simple_eq.
     iDestruct (heap_mapsto_lookup_1 with "Hσ Hmt") as %?; auto.
   Qed.
 
   Lemma heap_read_na σ l q v :
-    heap_ctx σ -∗ l ↦{q} v ==∗ ∃ n,
+    heap_ctx σ -∗ l ↦s{q} v ==∗ ∃ n,
       ⌜σ !! l = Some (RSt n, v)⌝ ∗
       heap_ctx (<[l:=(RSt (S n), v)]> σ) ∗
       ∀ σ2, heap_ctx σ2 ==∗ ∃ n2, ⌜σ2 !! l = Some (RSt (S n2), v)⌝ ∗
-        heap_ctx (<[l:=(RSt n2, v)]> σ2) ∗ l ↦{q} v.
+        heap_ctx (<[l:=(RSt n2, v)]> σ2) ∗ l ↦s{q} v.
   Proof.
     iDestruct 1 as (hF) "(Hσ & HhF & %)"; iIntros "Hmt".
-    rewrite heap_mapsto_eq.
+    rewrite heap_mapsto_simple_eq.
     iDestruct (heap_mapsto_lookup with "Hσ Hmt") as %[n Hσl]; eauto.
     iMod (heap_read_vs _ 0 1 with "Hσ Hmt") as "[Hσ Hmt]"; first done.
     iModIntro. iExists n; iSplit; [done|]. iSplitL "HhF Hσ".
@@ -525,24 +689,24 @@ Section heap.
   Qed.
 
   Lemma heap_write σ l v v' :
-    heap_ctx σ -∗ l ↦ v ==∗ heap_ctx (<[l:=(RSt 0, v')]> σ) ∗ l ↦ v'.
+    heap_ctx σ -∗ l ↦s v ==∗ heap_ctx (<[l:=(RSt 0, v')]> σ) ∗ l ↦s v'.
   Proof.
     iDestruct 1 as (hF) "(Hσ & HhF & %)". iIntros "Hmt".
-    rewrite heap_mapsto_eq.
+    rewrite heap_mapsto_simple_eq.
     iDestruct (heap_mapsto_lookup_1 with "Hσ Hmt") as %?; auto.
     iMod (heap_write_vs with "Hσ Hmt") as "[Hσ $]"; first done.
     iModIntro. iExists _. iFrame. eauto using heap_freeable_rel_stable.
   Qed.
 
   Lemma heap_write_na σ l v v' :
-    heap_ctx σ -∗ l ↦ v ==∗
+    heap_ctx σ -∗ l ↦s v ==∗
       ⌜σ !! l = Some (RSt 0, v)⌝ ∗
       heap_ctx (<[l:=(WSt, v)]> σ) ∗
       ∀ σ2, heap_ctx σ2 ==∗ ⌜σ2 !! l = Some (WSt, v)⌝ ∗
-        heap_ctx (<[l:=(RSt 0, v')]> σ2) ∗ l ↦ v'.
+        heap_ctx (<[l:=(RSt 0, v')]> σ2) ∗ l ↦s v'.
   Proof.
     iDestruct 1 as (hF) "(Hσ & HhF & %)"; iIntros "Hmt".
-    rewrite heap_mapsto_eq.
+    rewrite heap_mapsto_simple_eq.
     iDestruct (heap_mapsto_lookup_1 with "Hσ Hmt") as %?; eauto.
     iMod (heap_write_vs with "Hσ Hmt") as "[Hσ Hmt]"; first done.
     iModIntro. iSplit; [done|]. iSplitL "HhF Hσ".
